\chapter{Proofs}\label{AppendixProofs}
\begin{proof}[Proof of Lemma~\ref{lem:rq:quadestimate}]
  This proof is due to BÃ¶rm~\cite[70]{boerm}.

  Let $\alpha \in \C$. By using Lemma~\ref{lem:rq:properties} (ii) we
  obtain
  \begin{align*}
    \abs{\rq_{\mat{A}}(\vec{x}) - \lambda}
    &=
      \abs{\rq_{\mat{A} - \lambda \mat{I}}(\vec{x})}\\
    &=
      \abs{
      \frac{\langle \vec{x}, (\mat{A} - \lambda \mat{I}) \vec{x} \rangle}{\langle \vec{x}, \vec{x} \rangle}
      }\\
    &=
      \frac{
      \abs{
      \langle \vec{x}, (\mat{A} - \lambda \mat{I})(\vec{x} - \alpha \vec{v}) \rangle
      }
      }{
      \norm{x}^2
      }
    \\
    &=
      \frac{
      \abs{
      \langle {(\mat{A} - \lambda \mat{I})}^\ast \vec{x}, \vec{x} - \alpha \vec{v} \rangle
      }
      }{
      \norm{x}^2
      }
    \\
    &= 
      \frac{
      \abs{
      \langle {(\mat{A} - \lambda \mat{I})}^\ast(\vec{x} - \alpha \vec{v}), \vec{x} - \alpha \vec{v} \rangle
      }
      }{
      \norm{x}^2
      }
    \\
    &=
      \frac{
      \abs{
      \langle {\vec{x} - \alpha \vec{v}, (\mat{A} - \lambda \mat{I})} (\vec{x} - \alpha \vec{v}) \rangle
      }
      }{
      \norm{x}^2
      }
    \\
    &\le
      \frac{
      \norm{\vec{x} - \alpha \vec{v}} \norm{\mat{A} - \lambda \mat{I}} \norm{\vec{x} - \alpha \vec{v}}
      }{
      \norm{\vec{x}}^2
      }
    \\
    &=
      \norm{\mat{A} - \lambda \mat{I}} {\left(
      \frac{
      \norm{\vec{x} - \alpha \vec{v}}
      }{
      \norm{\vec{x}}
      }
      \right)}^2
  \end{align*}
\end{proof}
\todo{Finish proof (maybe in appendix?)}
%%% Local Variables:
%%% mode: latex
%%% TeX-master: "../main"
%%% End:
